{
    "@context": {
        "skos": "http://www.w3.org/2004/02/skos/core#",
        "og": "http://ogp.me/ns#",
        "dct": "http://purl.org/dc/terms/"
    },
    "@graph": [
        {
            "@id": "https://www.repostatus.org",
            "@type": "skos:ConceptScheme",
            "dct:title": "repostatus.org",
            "dct:description": "A standard to easily communicate to humans and machines the development/support and usability status of software repositories/projects.",
            "dct:creator": "Jason Antman"
        },
        {
            "@id": "https://www.repostatus.org/#abandoned",
            "@type": "skos:Concept",
            "skos:prefLabel": "Abandoned",
            "skos:definition": "Initial development has started, but there has not yet been a stable, usable release; the project has been abandoned and the author(s) do not intend on continuing development.",
            "skos:inScheme": "https://www.repostatus.org",
            "og:image": "https://www.repostatus.org/badges/latest/abandoned.svg"
        },
        {
            "@id": "https://www.repostatus.org/#active",
            "@type": "skos:Concept",
            "skos:prefLabel": "Active",
            "skos:definition": "The project has reached a stable, usable state and is being actively developed.",
            "skos:inScheme": "https://www.repostatus.org",
            "og:image": "https://www.repostatus.org/badges/latest/active.svg"
        },
        {
            "@id": "https://www.repostatus.org/#concept",
            "@type": "skos:Concept",
            "skos:prefLabel": "skos:Concept",
            "skos:definition": "Minimal or no implementation has been done yet, or the repository is only intended to be a limited example, demo, or proof-of-concept.",
            "skos:inScheme": "https://www.repostatus.org",
            "og:image": "https://www.repostatus.org/badges/latest/concept.svg"
        },
        {
            "@id": "https://www.repostatus.org/#inactive",
            "@type": "skos:Concept",
            "skos:prefLabel": "Inactive",
            "skos:definition": "The project has reached a stable, usable state but is no longer being actively developed; support/maintenance will be provided as time allows.",
            "skos:inScheme": "https://www.repostatus.org",
            "og:image": "https://www.repostatus.org/badges/latest/inactive.svg"
        },
        {
            "@id": "https://www.repostatus.org/#moved",
            "@type": "skos:Concept",
            "skos:prefLabel": "Moved",
            "skos:definition": "The project has been moved to a new location, and the version at that location should be considered authoritative.",
            "skos:inScheme": "https://www.repostatus.org",
            "og:image": "https://www.repostatus.org/badges/latest/moved.svg"
        },
        {
            "@id": "https://www.repostatus.org/#suspended",
            "@type": "skos:Concept",
            "skos:prefLabel": "Suspended",
            "skos:definition": "Initial development has started, but there has not yet been a stable, usable release; work has been stopped for the time being but the author(s) intend on resuming work.",
            "skos:inScheme": "https://www.repostatus.org",
            "og:image": "https://www.repostatus.org/badges/latest/suspended.svg"
        },
        {
            "@id": "https://www.repostatus.org/#unsupported",
            "@type": "skos:Concept",
            "skos:prefLabel": "Unsupported",
            "skos:definition": "The project has reached a stable, usable state but the author(s) have ceased all work on it. A new maintainer may be desired.",
            "skos:inScheme": "https://www.repostatus.org",
            "og:image": "https://www.repostatus.org/badges/latest/unsupported.svg"
        },
        {
            "@id": "https://www.repostatus.org/#wip",
            "@type": "skos:Concept",
            "skos:prefLabel": "WIP",
            "skos:altLabel": "Work in Progress",
            "skos:definition": "Initial development is in progress, but there has not yet been a stable, usable release suitable for the public.",
            "skos:inScheme": "https://www.repostatus.org",
            "og:image": "https://www.repostatus.org/badges/latest/wip.svg"
        }
  ]
}
